src/ReactorModel/Objects/Reactor/Practical.lean
@@ -1,8 +1,9 @@
 import ReactorModel.Objects.Reactor.Finite
+import ReactorModel.Objects.Reactor.Updatable
 import ReactorModel.Objects.Reactor.Proper
 
 namespace ReactorType
 
-class Practical (α) extends Finite α, Proper α  
+class Practical (α) extends Finite α, LawfulUpdatable α, Proper α  
 
 end ReactorType
