src/ReactorModel/Objects/Reactor/Theorems.lean
@@ -3,8 +3,7 @@ import ReactorModel.Objects.Reactor.Theorems.Basic
 import ReactorModel.Objects.Reactor.Theorems.Extensional
 import ReactorModel.Objects.Reactor.Theorems.FiniteUpdatable
 import ReactorModel.Objects.Reactor.Theorems.Indexable
+import ReactorModel.Objects.Reactor.Theorems.Practical
 import ReactorModel.Objects.Reactor.Theorems.Proper
 import ReactorModel.Objects.Reactor.Theorems.Readable
 import ReactorModel.Objects.Reactor.Theorems.WellFounded
-import ReactorModel.Objects.Reactor.Theorems.WellIndexable
-import ReactorModel.Objects.Reactor.Theorems.WellUpdatable
