src/ReactorModel/Objects/Reactor/Theorems/Indexable.lean
@@ -11,8 +11,8 @@ variable [Indexable α] {rtr rtr₁ : α}
 theorem unique (s₁ s₂ : StrictMember cpt i rtr) : s₁ = s₂ := by
   injection unique_ids.allEq (.strict s₁) (.strict s₂)
 
--- TODO: In both of the following theorems, the `final.nested` and `nested.final` cases could be 
---       removed if we have a theorem that establishes that for indexable reactor types, if two
+-- TODO: In all three of the following theorems, the `final.nested` and `nested.final` cases could 
+--       be removed if we have a theorem that establishes that for indexable reactor types, if two
 --       reactors are equivalent, then so are their membership witnesses.
 
 -- TODO: Note that both of the following theorems are almost identical. The only difference happens
@@ -50,6 +50,37 @@ theorem equiv_rcn_eq
   case nested.final h₁ s₁ _ _ h₂ =>
     injection (nested h₁ s₁).unique (final h₂ |>.fromEquiv $ ReactorType.Equivalent.symm e) 
 
+theorem lawfulMemUpdate_object_preserved 
+    (u : LawfulMemUpdate cpt i f rtr₁ rtr₂) (h : c ≠ cpt ∨ j ≠ i) (s₁ : StrictMember c j rtr₁)
+    (s₂ : StrictMember c j rtr₂) : s₁.object = s₂.object := by
+  induction s₁ generalizing rtr₂ <;> cases s₂ <;> simp [object]
+  case final.final h₁ _ h₂ =>
+    cases u
+    case final e => simp_all [e.valued h]
+    case nested e => simp_all [e (c := c) (.inl $ by simp)]
+  case nested.nested j₁ _ h₁ s₁ hi j₂ _ s₂ h₂ => 
+    have hj : j₁ = j₂ := by 
+      have hs := (nested h₁ s₁ |>.fromEquiv u.equiv).unique (nested h₂ s₂)
+      simp [fromEquiv] at hs
+      exact hs.left
+    subst hj
+    cases u
+    case final e => 
+      cases h₂ ▸ (e (c := .rtr) (j := j₁) (.inl $ by simp)) ▸ h₁
+      simp [s₁.unique s₂]
+    case nested j' _ _ u _ _ e =>
+      by_cases hj : j₁ = j'
+      case neg => 
+        cases h₂ ▸ (e (c := .rtr) (j := j₁) (.inr hj)) ▸ h₁
+        simp [s₁.unique s₂]
+      case pos => 
+        simp_all [hj]
+        exact hi (h₁ ▸ h₂ ▸ u) _
+  case final.nested h₁ _ _ s₂ h₂ =>
+    injection (final h₁ |>.fromEquiv u.equiv).unique (nested h₂ s₂)
+  case nested.final h₁ s₁ _ _ h₂ =>
+    injection (nested h₁ s₁).unique (final h₂ |>.fromEquiv $ ReactorType.Equivalent.symm u.equiv)     
+
 end StrictMember
 
 /- ---------------------------------------------------------------------------------------------- -/
@@ -69,6 +100,11 @@ theorem rtr_equiv (e : rtr₁ ≈ rtr₂) :
 theorem equiv_rcn_eq (e : rtr₁ ≈ rtr₂) :
     (m₁ : Member .rcn i rtr₁) → (m₂ : Member .rcn i rtr₂) → m₁.object = m₂.object 
   | strict s₁, strict s₂ => s₁.equiv_rcn_eq e s₂
+
+theorem lawfulMemUpdate_object_preserved 
+    (u : LawfulMemUpdate cpt i f rtr₁ rtr₂) (h : c ≠ cpt ∨ j ≠ i) :
+    (m₁ : Member c j rtr₁) → (m₂ : Member c j rtr₂) → m₁.object = m₂.object
+  | .strict s₁, .strict s₂ => s₁.lawfulMemUpdate_object_preserved u h s₂
 
 end Member
 
@@ -166,6 +202,7 @@ theorem obj?_none_to_get?_none {i : ID} (ho : rtr[cpt][i] = none) : rtr{cpt}{i} 
 
 end Indexable
 
+/- ---------------------------------------------------------------------------------------------- -/
 namespace Equivalent
 
 variable [Indexable α] {rtr₁ : α}
@@ -212,4 +249,68 @@ theorem obj?_rcn_eq (e : rtr₁ ≈ rtr₂) : rtr₁[.rcn] = rtr₂[.rcn] := by
     simp [ho₂, m₁.equiv_rcn_eq e m₂]
 
 end Equivalent
+
+/- ---------------------------------------------------------------------------------------------- -/
+namespace LawfulMemUpdate
+
+open Indexable
+variable [Indexable α] {rtr₁ : α}
+
+theorem obj?_some₁ (u : LawfulMemUpdate cpt i f rtr₁ rtr₂) : ∃ o, rtr₁[cpt][i] = some o := by
+  induction u 
+  case final           => exact ⟨_, get?_some_to_obj?_some ‹_›⟩
+  case nested h _ _ hi => exact ⟨_, obj?_some_nested h hi.choose_spec⟩
+
+theorem obj?_some₂ (u : LawfulMemUpdate cpt i f rtr₁ rtr₂) : ∃ o, rtr₂[cpt][i] = some o := by
+  induction u 
+  case final         => exact ⟨_, get?_some_to_obj?_some ‹_›⟩
+  case nested h _ hi => exact ⟨_, obj?_some_nested h hi.choose_spec⟩
+
+theorem obj?_some_iff (u : LawfulMemUpdate cpt i f rtr₁ rtr₂) : 
+    (∃ o, rtr₁[c][j] = some o) ↔ (∃ o, rtr₂[c][j] = some o) :=
+  Equivalent.obj?_some_iff u.equiv
+
+theorem obj?_none_iff (u : LawfulMemUpdate cpt i f rtr₁ rtr₂) : 
+    (rtr₁[c][j] = none) ↔ (rtr₂[c][j] = none) :=
+  Equivalent.obj?_none_iff u.equiv
+
+theorem obj?_preserved (u : LawfulMemUpdate cpt i f rtr₁ rtr₂) (h : c ≠ cpt ∨ j ≠ i) : 
+    rtr₂[c][j] = rtr₁[c][j] := by
+  cases ho₁ : rtr₁[c][j]
+  case none => simp [obj?_none_iff u |>.mp ho₁]
+  case some =>
+    have ⟨_, ho₂⟩ := obj?_some_iff u |>.mp ⟨_, ho₁⟩ 
+    have ⟨m₁⟩ := Object.iff_obj?_some.mpr ho₁
+    have ⟨m₂⟩ := Object.iff_obj?_some.mpr ho₂
+    simp [ho₂, m₁.lawfulMemUpdate_object_preserved u h m₂]
+
+theorem obj?_updated (u : LawfulMemUpdate cpt i f rtr₁ rtr₂) : 
+    rtr₂[cpt][i] = f <$> rtr₁[cpt][i] := by
+  induction u
+  case final h₁ h₂ => 
+    rw [get?_some_to_obj?_some h₁, get?_some_to_obj?_some h₂, Option.map_some]
+  case nested h₁ h₂ u hi =>
+    have ⟨_, h₁'⟩ := u.obj?_some₁
+    have ⟨_, h₂'⟩ := u.obj?_some₂
+    rw [obj?_some_nested h₁ h₁', obj?_some_nested h₂ h₂']
+    exact h₁' ▸ h₂' ▸ hi
+
+end LawfulMemUpdate
+
+/- ---------------------------------------------------------------------------------------------- -/
+namespace LawfulUpdate
+
+open Indexable
+variable [Indexable α] {rtr₁ : α}
+
+theorem obj?_preserved (h : c ≠ cpt ∨ j ≠ i) : 
+    (LawfulUpdate cpt i f rtr₁ rtr₂) → rtr₂[c][j] = rtr₁[c][j]
+  | update u   => u.obj?_preserved h
+  | notMem _ h => h ▸ rfl
+
+theorem obj?_updated : (LawfulUpdate cpt i f rtr₁ rtr₂) → rtr₂[cpt][i] = f <$> rtr₁[cpt][i]
+  | update u   => u.obj?_updated
+  | notMem h e => by subst e; simp [member_isEmpty_obj?_none h]
+
+end LawfulUpdate
 end ReactorType
