src/ReactorModel/Objects/Reactor/Theorems/Practical.lean
@@ -1,0 +1,17 @@
+import ReactorModel.Objects.Reactor.Practical
+import ReactorModel.Objects.Reactor.Theorems.Accessible
+import ReactorModel.Objects.Reactor.Theorems.Proper
+
+namespace ReactorType
+
+instance [Practical α] : Accessible α where
+  unique_ids := Practical.toProper.unique_ids
+
+variable [Practical α] {rtr : α}
+
+open Updatable in
+theorem LawfulUpdatable.update_ne_comm (h : cpt₁ ≠ cpt₂ ∨ i₁ ≠ i₂):
+    update (update rtr cpt₁ i₁ f₁) cpt₂ i₂ f₂ = update (update rtr cpt₂ i₂ f₂) cpt₁ i₁ f₁ :=
+  LawfulUpdate.ne_comm (lawful ..) (lawful ..) (lawful ..) (lawful ..) h
+
+end ReactorType
