src/ReactorModel/Objects/Reactor/Theorems/WellFounded.lean
@@ -7,88 +7,14 @@ noncomputable section
 open Classical
 
 namespace ReactorType
-namespace Equivalent
-
-variable [WellFounded α]
-
-@[refl]
-theorem refl (rtr : α) : rtr ≈ rtr := by
-  induction rtr using WellFounded.induction
-  case nested hi =>
-    constructor <;> (intros; simp_all)
-    exact hi _ _ ‹_›  
-
-instance : Equivalence ((· : α) ≈ ·) := 
-  { refl, symm, trans }
-
-end Equivalent
-
-theorem LawfulMemUpdate.equiv [WellFounded α] {rtr₁ : α}
-    (u : LawfulMemUpdate cpt i f rtr₁ rtr₂) : rtr₁ ≈ rtr₂ := by
-  induction u <;> constructor
-  case final.mem_get?_iff e h₁ h₂ =>
-    intro c j
-    by_cases hc : c = cpt <;> try subst hc
-    case neg => exact e.mem_iff (.inl hc)
-    case pos =>
-      by_cases hj : j = i <;> try subst hj
-      case neg => exact e.mem_iff (.inr hj)
-      case pos => simp [Partial.mem_iff, h₁, h₂]
-  case final.get?_rcn_some_eq e _ _ =>
-    intro j _ _ h₁ h₂
-    have h := e (c := .rcn) (j := j) (.inl $ by simp)
-    simp_all
-  case final.get?_rtr_some_equiv e _ _ =>
-    intro j _ _ h₁ h₂
-    have h := e (c := .rtr) (j := j) (.inl $ by simp)
-    simp_all
-    apply Equivalent.refl
-  case nested.mem_get?_iff j _ _ _ _ e h₁ h₂ _ _ =>
-    intro c j'
-    by_cases hc : c = .rtr <;> try subst hc
-    case neg => exact e.mem_iff (.inl hc)
-    case pos => 
-      by_cases hj : j' = j <;> try subst hj
-      case neg => exact e.mem_iff (.inr hj)
-      case pos => simp [Partial.mem_iff, h₁, h₂]
-  case nested.get?_rcn_some_eq e h₁ h₂ _ _ =>
-    intro j _ _ h₁ h₂
-    have h := e (c := .rcn) (j := j) (.inl $ by simp)
-    simp_all
-  case nested.get?_rtr_some_equiv j _ _ _ _ e _ _ _ hi =>
-    intro j' n₁' n₂' h₁' h₂'
-    by_cases hj : j' = j <;> try subst hj
-    case pos => simp_all; assumption
-    case neg => 
-      have := e (c := .rtr) (j := j') (.inr hj)
-      simp_all
-      apply Equivalent.refl
-
-theorem LawfulUpdate.equiv [WellFounded α] {rtr₁ : α} :
-    (LawfulUpdate cpt i f rtr₁ rtr₂) → rtr₁ ≈ rtr₂
-  | notMem _ h => h ▸ (.refl _)
-  | update u   => u.equiv
-
 namespace StrictMember
 
 variable [WellFounded α] {rtr rtr₁ : α}
 
-def fromLawfulMemUpdate {rtr₁ : α} : 
-    (StrictMember c j rtr₂) → (LawfulMemUpdate cpt i f rtr₁ rtr₂) → StrictMember c j rtr₁
-  | final h, u               => final $ (Equivalent.get?_some_iff u.equiv).mpr ⟨_, h⟩ |>.choose_spec
-  | nested h s, .final e _ _ => nested (h ▸ e (.inl $ by simp)) s 
-  | nested h s (j := j₂), .nested e h₁ h₂ u (j := j₁) =>
-      if hj : j₂ = j₁ 
-      then nested h₁ $ fromLawfulMemUpdate ((Option.some_inj.mp $ h₂ ▸ hj ▸ h) ▸ s) u
-      else nested (h ▸ e $ .inr hj) s 
-
-def fromLawfulUpdate (s : StrictMember c j rtr₂) : 
-    (LawfulUpdate cpt i f rtr₁ rtr₂) → StrictMember c j rtr₁
-  | .notMem _ h => h ▸ s
-  | .update u   => s.fromLawfulMemUpdate u
-
 namespace Equivalent
 
+-- TODO: Adjust the definition of Member Equivalence to include a refl case, so you can remove the 
+--       requirement of wellfoundedness. Then you can also move all of the theorems below.
 @[refl]
 theorem refl (s : StrictMember cpt i rtr) : Equivalent s s := by
   induction rtr using WellFounded.induction
@@ -118,22 +44,9 @@ theorem fromLawfulUpdate (u : LawfulUpdate cpt i f rtr₁ rtr₂) (s : StrictMem
 end Equivalent
 end StrictMember
 
--- TODO: All of the definitions/theorems in this namespace could be lifted pretty mechanically from
---       `StrictMember`.
 namespace Member
 
 variable [WellFounded α] {rtr rtr₁ : α}
-
-def fromLawfulMemUpdate (m : Member c j rtr₂) (u : LawfulMemUpdate cpt i f rtr₁ rtr₂) : 
-    Member c j rtr₁ :=
-  match m with
-  | root => root 
-  | strict s => s.fromLawfulMemUpdate u
-
-def fromLawfulUpdate (m : Member c j rtr₂) (u : LawfulUpdate cpt i f rtr₁ rtr₂) : Member c j rtr₁ :=
-  match m with
-  | root => root
-  | strict s => s.fromLawfulUpdate u
 
 namespace Equivalent
 
